LambdaLab.lean
@@ -84,5 +84,3 @@ import LambdaLab.Parser.Truncation
 import LambdaLab.Parser.Truncation.Mixfix
 import LambdaLab.Stlc.Named.Lang
 import LambdaLab.Stlc.Named.Mvars
-import LambdaLab.Stlc.Named.Solving
-import LambdaLab.Stlc.Named.Inference
